Build fixes + generalise sub_borrow proof

dist/gcc-compatible/Hacl_IntTypes_Intrinsics_128.h
@@ -22,8 +22,8 @@
  */
 
 
-#ifndef __Hacl_IntTypes_Intrinsics_H
-#define __Hacl_IntTypes_Intrinsics_H
+#ifndef __Hacl_IntTypes_Intrinsics_128_H
+#define __Hacl_IntTypes_Intrinsics_128_H
 
 #if defined(__cplusplus)
 extern "C" {
@@ -39,44 +39,32 @@ extern "C" {
 
 #include "Hacl_Kremlib.h"
 
-static inline uint32_t
-Hacl_IntTypes_Intrinsics_add_carry_u32(uint32_t cin, uint32_t x, uint32_t y, uint32_t *r)
+static inline uint64_t
+Hacl_IntTypes_Intrinsics_128_add_carry_u64(uint64_t cin, uint64_t x, uint64_t y, uint64_t *r)
 {
-  uint64_t res = (uint64_t)x + (uint64_t)cin + (uint64_t)y;
-  uint32_t c = (uint32_t)(res >> (uint32_t)32U);
-  r[0U] = (uint32_t)res;
-  return c;
-}
-
-static inline uint32_t
-Hacl_IntTypes_Intrinsics_sub_borrow_u32(uint32_t cin, uint32_t x, uint32_t y, uint32_t *r)
-{
-  uint64_t res = (uint64_t)x - (uint64_t)y - (uint64_t)cin;
-  uint32_t c = (uint32_t)(res >> (uint32_t)32U) & (uint32_t)1U;
-  r[0U] = (uint32_t)res;
+  FStar_UInt128_uint128
+  res =
+    FStar_UInt128_add_mod(FStar_UInt128_add_mod(FStar_UInt128_uint64_to_uint128(x),
+        FStar_UInt128_uint64_to_uint128(cin)),
+      FStar_UInt128_uint64_to_uint128(y));
+  uint64_t c = FStar_UInt128_uint128_to_uint64(FStar_UInt128_shift_right(res, (uint32_t)64U));
+  r[0U] = FStar_UInt128_uint128_to_uint64(res);
   return c;
 }
 
 static inline uint64_t
-Hacl_IntTypes_Intrinsics_add_carry_u64(uint64_t cin, uint64_t x, uint64_t y, uint64_t *r)
+Hacl_IntTypes_Intrinsics_128_sub_borrow_u64(uint64_t cin, uint64_t x, uint64_t y, uint64_t *r)
 {
-  uint64_t res = x + cin + y;
-  uint64_t
-  c = (~FStar_UInt64_gte_mask(res, x) | (FStar_UInt64_eq_mask(res, x) & cin)) & (uint64_t)1U;
-  r[0U] = res;
-  return c;
-}
-
-static inline uint64_t
-Hacl_IntTypes_Intrinsics_sub_borrow_u64(uint64_t cin, uint64_t x, uint64_t y, uint64_t *r)
-{
-  uint64_t res = x - y - cin;
+  FStar_UInt128_uint128
+  res =
+    FStar_UInt128_sub_mod(FStar_UInt128_sub_mod(FStar_UInt128_uint64_to_uint128(x),
+        FStar_UInt128_uint64_to_uint128(y)),
+      FStar_UInt128_uint64_to_uint128(cin));
   uint64_t
   c =
-    ((FStar_UInt64_gte_mask(res, x) & ~FStar_UInt64_eq_mask(res, x))
-    | (FStar_UInt64_eq_mask(res, x) & cin))
+    FStar_UInt128_uint128_to_uint64(FStar_UInt128_shift_right(res, (uint32_t)64U))
     & (uint64_t)1U;
-  r[0U] = res;
+  r[0U] = FStar_UInt128_uint128_to_uint64(res);
   return c;
 }
 
@@ -84,5 +72,5 @@ Hacl_IntTypes_Intrinsics_sub_borrow_u64(uint64_t cin, uint64_t x, uint64_t y, ui
 }
 #endif
 
-#define __Hacl_IntTypes_Intrinsics_H_DEFINED
+#define __Hacl_IntTypes_Intrinsics_128_H_DEFINED
 #endif
