code/fallback/Hacl.IntTypes.Intrinsics.fst
@@ -9,21 +9,7 @@ open Lib.Buffer
 
 open FStar.Mul
 
-#set-options "--fuel 0 --ifuel 0 --z3rlimit 100"
-
-
-inline_for_extraction noextract
-let add_carry_st (t:inttype{t = U32 \/ t = U64}) =
-    cin:uint_t t SEC
-  -> x:uint_t t SEC
-  -> y:uint_t t SEC
-  -> r:lbuffer (uint_t t SEC) (size 1) ->
-  Stack (uint_t t SEC)
-  (requires fun h -> live h r /\ v cin <= 1)
-  (ensures  fun h0 c h1 ->
-    modifies1 r h0 h1 /\ v c <= 1 /\
-    (let r = Seq.index (as_seq h1 r) 0 in
-    v r + v c * pow2 (bits t) == v x + v y + v cin))
+#set-options "--fuel 0 --ifuel 0 --z3rlimit 500"
 
 inline_for_extraction noextract
 val cast_to : t:inttype{t = U32 \/ t = U64} ->
@@ -46,6 +32,19 @@ let cast_from t t' =
   | U128 -> cast U64 SEC
 
 inline_for_extraction noextract
+let add_carry_st (t:inttype{t = U32 \/ t = U64}) =
+    cin:uint_t t SEC
+  -> x:uint_t t SEC
+  -> y:uint_t t SEC
+  -> r:lbuffer (uint_t t SEC) (size 1) ->
+  Stack (uint_t t SEC)
+  (requires fun h -> live h r /\ v cin <= 1)
+  (ensures  fun h0 c h1 ->
+    modifies1 r h0 h1 /\ v c <= 1 /\
+    (let r = Seq.index (as_seq h1 r) 0 in
+    v r + v c * pow2 (bits t) == v x + v y + v cin))
+
+inline_for_extraction noextract
 val add_carry:
   t:inttype{t = U32 \/ t = U64} ->
   t':inttype{if t = U32 then t' = U64 else t' = U128} ->
@@ -60,6 +59,15 @@ let add_carry t t' shift_bits cin x y r =
 val add_carry_u32: add_carry_st U32
 let add_carry_u32 = add_carry U32 U64 32ul
 
+
+inline_for_extraction noextract
+val to_uint : t:inttype{t = U32 \/ t = U64} ->
+  (n:range_t t -> u:int_t t SEC{v u == n})
+let to_uint t =
+  match t with
+  | U32 -> u32
+  | U64 -> u64
+
 inline_for_extraction noextract
 let sub_borrow_st (t:inttype{t = U32 \/ t = U64}) =
     cin:uint_t t SEC
@@ -73,30 +81,44 @@ let sub_borrow_st (t:inttype{t = U32 \/ t = U64}) =
     (let r = Seq.index (as_seq h1 r) 0 in
     v r - v c * pow2 (bits t) == v x - v y - v cin))
 
-val sub_borrow_u32: sub_borrow_st U32
-let sub_borrow_u32 cin x y r =
-  let res = to_u64 x -. to_u64 y -. to_u64 cin in
-  assert (v res == ((v x - v y) % pow2 64 - v cin) % pow2 64);
-  Math.Lemmas.lemma_mod_add_distr (- v cin) (v x - v y) (pow2 64);
-  assert (v res == (v x - v y - v cin) % pow2 64);
+#push-options "--z3rlimit 1000 --max_fuel 1"
 
-  assert (v res % pow2 32 = (v x - v y - v cin) % pow2 64 % pow2 32);
-  Math.Lemmas.pow2_modulo_modulo_lemma_1 (v x - v y - v cin) 32 64;
-  assert (v res % pow2 32 = (v x - v y - v cin) % pow2 32);
+inline_for_extraction noextract
+val sub_borrow:
+  t:inttype{t = U32 \/ t = U64} ->
+  t':inttype{if t = U32 then t' = U64 else t' = U128} ->
+  shift_bits:UInt32.t{if t = U32 then shift_bits == 32ul else shift_bits == 64ul} ->
+  p:UInt32.t{if t = U32 then p == 64ul else p == 128ul} ->
+  sub_borrow_st t
+let sub_borrow t t' shift_bits p cin x y r =
+  let res = cast_to t t' x -. cast_to t t' y -. cast_to t t' cin in
+  assert (v res == ((v x - v y) % pow2 (v p) - v cin) % pow2 (v p));
+  Math.Lemmas.lemma_mod_add_distr (- v cin) (v x - v y) (pow2 (v p));
+  assert (v res == (v x - v y - v cin) % pow2 (v p));
 
-  let c = to_u32 (res >>. 32ul) &. u32 1 in
+  assert (v res % pow2 (v shift_bits) = (v x - v y - v cin) % pow2 (v p) % pow2 (v shift_bits));
+  Math.Lemmas.pow2_modulo_modulo_lemma_1 (v x - v y - v cin) (v shift_bits) (v p);
+  assert (v res % pow2 (v shift_bits) = (v x - v y - v cin) % pow2 (v shift_bits));
+
+  let c = cast_from t' t (res >>. shift_bits) &. (to_uint t 1) in
   assert_norm (pow2 1 = 2);
-  mod_mask_lemma (to_u32 (res >>. 32ul)) 1ul;
-  assert (v ((mk_int #U32 #SEC 1 <<. 1ul) -! mk_int 1) == 1);
-  assert (v c = v res / pow2 32 % pow2 1);
+  mod_mask_lemma (cast_from t' t (res >>. shift_bits)) 1ul;
+  assert (v ((mk_int #t #SEC 1 <<. 1ul) -! mk_int 1) == 1);
+  assert (v c = v res / pow2 (v shift_bits) % pow2 1);
 
-  r.(0ul) <- to_u32 res;
+  r.(0ul) <- cast_from t' t res;
   assert (v c = (if 0 <= v x - v y - v cin then 0 else 1));
   c
 
+val sub_borrow_u32: sub_borrow_st U32
+let sub_borrow_u32 = sub_borrow U32 U64 32ul 64ul
+
 
 (* Fallback versions of add_carry_u64 and sub_borrow_u64 for platforms which
-   don't support uint128 *)
+   don't support uint128.
+   The names Hacl.IntTypes.Intrinsics.add_carry_u64 and sub_borrow_u64 must not
+   be changed because they are hardcoded in KreMLin for extracting wasm code
+   which uses these intrinsics. *)
 inline_for_extraction noextract
 val add_carry_fallback: #t:inttype{t = U32 \/ t = U64} -> add_carry_st t
 let add_carry_fallback #t cin x y r =
@@ -108,8 +130,8 @@ let add_carry_fallback #t cin x y r =
   logand_mask (logor (lt_mask res x) (logand (eq_mask res x) cin)) (uint #t 1) 1;
   c
 
-val add_carry_u64_fallback: add_carry_st U64
-let add_carry_u64_fallback cin x y r = add_carry_fallback #U64 cin x y r
+val add_carry_u64: add_carry_st U64
+let add_carry_u64 cin x y r = add_carry_fallback #U64 cin x y r
 
 inline_for_extraction noextract
 val sub_borrow_fallback: #t:inttype{t = U32 \/ t = U64} -> sub_borrow_st t
@@ -122,5 +144,5 @@ let sub_borrow_fallback #t cin x y r =
   r.(0ul) <- res;
   c
 
-val sub_borrow_u64_fallback: sub_borrow_st U64
-let sub_borrow_u64_fallback cin x y r = sub_borrow_fallback #U64 cin x y r
+val sub_borrow_u64: sub_borrow_st U64
+let sub_borrow_u64 cin x y r = sub_borrow_fallback #U64 cin x y r
